Clean/Circuit/Lawful.lean
@@ -153,11 +153,14 @@ def Circuit.constant_output (circuit : α → Circuit F β) [Inhabited α] :=
 -- characterize various properties of (lawful) circuits
 
 namespace Circuit
-variable {env : Environment F} {n : ℕ} {prop : Operations.Condition F}
+variable {n : ℕ} {prop : Operations.Condition F}
 
 @[reducible, circuit_norm]
 def forAll (circuit : Circuit F α) (prop : Operations.Condition F) (n : ℕ) :=
   (circuit.operations n).forAll n prop
+
+lemma forAll_def {circuit : Circuit F α} {n : ℕ} :
+  circuit.forAll prop n ↔ (circuit.operations n).forAll n prop := by rfl
 
 theorem bind_forAll {f : Circuit F α} {g : α → Circuit F β} :
   (f >>= g).forAll prop n ↔
@@ -169,5 +172,21 @@ theorem bind_forAll {f : Circuit F α} {g : α → Circuit F β} :
 theorem bind_forAll_lawful {f : Circuit F α} {g : α → Circuit F β} (f_lawful: LawfulCircuit f) :
   (f >>= g).forAll prop n ↔ f.forAll prop n ∧ (g (f.output n)).forAll prop (n + f.local_length n) := by
   rw [bind_forAll, ←f_lawful.offset_consistent]
+
+theorem constraints_hold.soundness_iff_forAll' {env : Environment F} {circuit : Circuit F α} {n : ℕ} :
+  constraints_hold.soundness env (circuit.operations n) ↔ circuit.forAll {
+    assert _ e := env e = 0,
+    lookup _ l := l.table.contains (l.entry.map env),
+    subcircuit _ _ s := s.soundness env
+  } n := by
+  rw [forAll_def, constraints_hold.soundness_iff_forAll _ _ n]
+
+theorem constraints_hold.completeness_iff_forAll' {env : Environment F} {circuit : Circuit F α} {n : ℕ} :
+  constraints_hold.completeness env (circuit.operations n) ↔ circuit.forAll {
+    assert _ e := env e = 0,
+    lookup _ l := l.table.contains (l.entry.map env),
+    subcircuit _ _ s := s.completeness env
+  } n := by
+  rw [forAll_def, constraints_hold.completeness_iff_forAll _ _ n]
 
 end Circuit
